Bdd/DecisionTree.lean
@@ -1,0 +1,39 @@
+import Mathlib.Data.Vector.Basic
+
+inductive DecisionTree n where
+  | leaf   : Bool  → DecisionTree _
+  | branch : Fin n → DecisionTree n → DecisionTree n → DecisionTree n
+deriving DecidableEq
+
+namespace DecisionTree
+
+def evaluate : DecisionTree n → Vector Bool n → Bool
+  | leaf b, _ => b
+  | branch j l h, v => if v[j] then h.evaluate v else l.evaluate v
+
+def size {n} : DecisionTree n → Nat
+  | leaf _ => 0
+  | branch _ l h => 1 + l.size + h.size
+
+inductive usesVar (i : Fin n) : DecisionTree n → Prop where
+  | here : usesVar i (.branch i _ _)
+  | low : usesVar i l → usesVar i (.branch _ l _)
+  | high : usesVar i h → usesVar i (.branch _ _ h)
+
+lemma usesVar_iff (i : Fin n) (T : DecisionTree n) :
+    T.usesVar i ↔ (∃ i' l h, T = .branch i' l h ∧ (i = i' ∨ l.usesVar i ∨ h.usesVar i)) := by
+  constructor
+  · intro h
+    cases h with
+    | here => simp
+    | low hl => simp [hl]
+    | high hh => simp [hh]
+  · rintro ⟨i', l, h, h1, h2⟩
+    cases h2 with
+    | inl => simp_all [usesVar.here]
+    | inr h2 =>
+      cases h2 with
+      | inl => simp_all [usesVar.low]
+      | inr => simp_all [usesVar.high]
+
+end DecisionTree
