Bdd/Evaluate.lean
@@ -1,0 +1,32 @@
+import Bdd.Basic
+
+namespace Evaluate
+
+def evaluate (O : OBdd n m) : Vector Bool n → Bool := fun I ↦
+  match h : O.1.root with
+  | .terminal b => b
+  | .node j => if I[O.1.heap[j].var] then evaluate (O.high h) I else evaluate (O.low h) I
+termination_by O
+
+lemma evaluate_evaluate {O : OBdd n m }: evaluate O = O.evaluate := by
+  ext I
+  unfold evaluate
+  split
+  next b hb => simp [OBdd.evaluate_terminal' hb]
+  next j hj =>
+    have := evaluate_evaluate (O := O.low hj)
+    have := evaluate_evaluate (O := O.high hj)
+    simp [OBdd.evaluate_node'' hj, *]
+termination_by O
+
+lemma evaluate_terminal {O : OBdd n m} : O.1.root = .terminal b → evaluate O = Function.const _ b := by
+  rw [evaluate_evaluate]
+  exact OBdd.evaluate_terminal'
+
+lemma evaluate_node {O : OBdd n m} (h : O.1.root = .node j) :
+    evaluate O = fun I ↦ if I[O.1.heap[j].var] then evaluate (O.high h) I else evaluate (O.low h) I := by
+  rw [evaluate_evaluate]
+  rw [OBdd.evaluate_node'' h]
+  simp [evaluate_evaluate]
+
+end Evaluate
