Bdd/Lift.lean
@@ -1,0 +1,247 @@
+import Bdd.Basic
+
+namespace Lift
+
+
+@[simp]
+private def lift_node : n ≤ n' → Node n m → Node n' m := fun h N ↦ ⟨⟨N.var.1, by exact Fin.val_lt_of_le N.var h⟩, N.low, N.high⟩
+
+private lemma lift_node_trivial_eq {n n' m : Nat} {h : n = n'} {N : Node n m} : lift_node (n' := n') (by rw [h]) N = h ▸ N := by
+  subst h
+  simp_all
+
+@[simp]
+private def lift_heap : n ≤ n' → Vector (Node n m) m → Vector (Node n' m) m := fun h v ↦ Vector.map (lift_node h) v
+
+@[simp]
+def lift : n ≤ n' → Bdd n m → Bdd n' m := fun h B ↦ ⟨lift_heap h B.heap, B.root⟩
+
+private lemma lift_edge_iff {h : n ≤ n'} {B : Bdd n m} {p q : Pointer m} :
+    Edge B.heap p q ↔ Edge (lift h B).heap p q := by
+  constructor
+  · intro e
+    cases e with
+    | low  _ => left;  simpa
+    | high _ => right; simpa
+  · intro e
+    cases e with
+    | low  _ => left;  simp_all
+    | high _ => right; simp_all
+
+private lemma lift_reachable_iff {h : n ≤ n'} {B : Bdd n m} {p : Pointer m} :
+    Pointer.Reachable B.heap B.root p ↔ Pointer.Reachable (lift h B).heap (lift h B).root p := by
+  constructor
+  · intro r
+    induction r with
+    | refl => left
+    | tail _ e ih =>
+      right
+      · exact ih
+      · exact (lift_edge_iff.mp e)
+  · intro r
+    induction r with
+    | refl => left
+    | tail _ e ih =>
+      right
+      · exact ih
+      · exact (lift_edge_iff.mpr e)
+
+private lemma lift_preserves_MayPrecede {h : n ≤ n'} {B : Bdd n m} {p q : Pointer m} :
+    Pointer.MayPrecede (lift h B).heap p q ↔ Pointer.MayPrecede B.heap p q := by
+  constructor
+  · intro hm
+    cases p with
+    | terminal _ =>
+      absurd hm
+      exact Pointer.not_terminal_MayPrecede
+    | node j =>
+      cases q with
+      | terminal _ =>
+        apply Pointer.MayPrecede_node_terminal
+      | node j' =>
+        simp only [Pointer.MayPrecede, Nat.succ_eq_add_one, lift, lift_heap, Pointer.toVar_node_eq, Fin.getElem_fin, lift_node] at hm
+        apply (Fin.natCast_lt_natCast (by omega) (by omega)).mp at hm
+        simp only [Pointer.MayPrecede, Nat.succ_eq_add_one, Pointer.toVar_node_eq, Fin.getElem_fin]
+        aesop
+  · intro hm
+    cases p with
+    | terminal _ =>
+      absurd hm
+      exact Pointer.not_terminal_MayPrecede
+    | node j =>
+      cases q with
+      | terminal _ =>
+        apply Pointer.MayPrecede_node_terminal
+      | node j' =>
+        simp only [Pointer.MayPrecede, Nat.succ_eq_add_one, Pointer.toVar_node_eq, Fin.getElem_fin] at hm
+        simp only [Pointer.MayPrecede, Nat.succ_eq_add_one, lift, lift_heap, Pointer.toVar_node_eq, Fin.getElem_fin, lift_node]
+        simp_all only [Fin.coe_eq_castSucc, Fin.castSucc_lt_castSucc_iff, Vector.getElem_map, lift_node]
+        refine (Fin.natCast_lt_natCast ?_ ?_).mpr ?_ <;> omega
+
+private lemma lift_preserves_RelevantEdge {h : n ≤ n'} {B : Bdd n m} {p q : Pointer m} :
+    ( ∃ (hp : Pointer.Reachable (lift h B).heap (lift h B).root p)
+        (hq : Pointer.Reachable (lift h B).heap (lift h B).root q), Bdd.RelevantEdge (lift h B) ⟨p, hp⟩ ⟨q, hq⟩) ↔
+    ( ∃ (hp : Pointer.Reachable B.heap B.root p)
+        (hq : Pointer.Reachable B.heap B.root q), Bdd.RelevantEdge B ⟨p, hp⟩ ⟨q, hq⟩) := by
+  constructor
+  · rintro ⟨hp, hq, hr⟩
+    use (lift_reachable_iff.mpr hp)
+    use (lift_reachable_iff.mpr hq)
+    cases hr with
+    | low  hl => simp at hl; left ; assumption
+    | high hh => simp at hh; right; assumption
+  · rintro ⟨hp, hq, hr⟩
+    use (lift_reachable_iff.mp hp)
+    use (lift_reachable_iff.mp hq)
+    cases hr with
+    | low  hl => simp at hl; left ; simpa
+    | high hh => simp at hh; right; simpa
+
+lemma lift_ordered {h : n ≤ n'} {B : Bdd n m} : B.Ordered → (lift h B).Ordered := by
+  rintro ho ⟨x, hx⟩ ⟨y, hy⟩ e
+  apply lift_preserves_MayPrecede.mpr
+  exact ho (lift_preserves_RelevantEdge.mp ⟨hx, hy, e⟩).2.2
+
+def olift : n ≤ n' → OBdd n m → OBdd n' m := fun h O ↦ ⟨(lift h O.1), lift_ordered O.2⟩
+
+@[simp]
+lemma olift_trivial_eq {h : n = n'} {O : OBdd n m} : (olift (n' := n') (by rw [h]) O) = h ▸ O := by
+  rcases O with ⟨⟨M, r⟩, o⟩
+  simp only [olift, lift, lift_heap]
+  congr
+  · have : (lift_node (Eq.mpr (id (congrArg (fun _a ↦ _a ≤ n') h)) (le_refl n'))) = fun (x : Node n m) ↦ h ▸ x := by
+      ext
+      exact lift_node_trivial_eq
+    rw [this]
+    subst h
+    simp only
+    rcases M with ⟨V, l⟩
+    simp [Vector.map, List.map_id_fun', id_eq]
+  · subst h
+    simp
+
+private lemma lift_preserves_root {h : n ≤ n'} {B : Bdd n m} : (lift h B).root = B.root := by simp
+
+@[simp]
+private lemma olift_preserves_root {h : n ≤ n'} {O : OBdd n m} : (olift h O).1.root = O.1.root := lift_preserves_root
+
+private lemma olift_low {h : n ≤ n'} {O : OBdd n m} {j : Fin m} (hr : O.1.root = .node j): (olift h O).low hr = olift h (O.low hr) := by
+  simp only [OBdd.low, olift, lift, lift_heap]
+  simp_rw [Bdd.low_heap_eq_heap]
+  simp_rw [hr]
+  simp [Bdd.low]
+
+private lemma olift_high {h : n ≤ n'} {O : OBdd n m} {j : Fin m} (hr : O.1.root = .node j): (olift h O).high hr = olift h (O.high hr) := by
+  simp only [OBdd.high, olift, lift, lift_heap]
+  simp_rw [Bdd.high_heap_eq_heap]
+  simp_rw [hr]
+  simp [Bdd.high]
+
+private lemma NoRedundancy_of_olift {h : n ≤ n'} {O : OBdd n m} : O.1.NoRedundancy → (olift h O).1.NoRedundancy := by
+  rintro hnr ⟨p, hp⟩ contra
+  simp only at contra
+  cases p_def : p with
+  | terminal _ =>
+    cases contra with
+    | red _ => contradiction
+  | node j =>
+    rw [p_def] at contra
+    cases contra with
+    | red red =>
+      simp only [olift, lift, lift_heap, Fin.getElem_fin, lift_node] at red
+      apply hnr ⟨p, lift_reachable_iff.mpr hp⟩
+      simp_rw [p_def]
+      constructor
+      simp_all
+
+-- FIXME: Move to DecisionTree.lean
+def tlift : n ≤ n' → DecisionTree n → DecisionTree n'
+  | _, .leaf b => .leaf b
+  | e, .branch j l h => .branch ⟨j.1, by omega⟩ (tlift e l) (tlift e h)
+
+lemma tlift_injective {n n' : Nat} {h : n ≤ n'} : Function.Injective (tlift h) := by
+  intro x y hxy
+  cases x with
+  | leaf _ =>
+    cases y with
+    | leaf _ => simp only [tlift] at hxy; simp_all
+    | branch _ _ _ => contradiction
+  | branch _ _ _ =>
+    cases y with
+    | leaf _ => contradiction
+    | branch _ _ _ =>
+      simp only [tlift] at hxy
+      injection hxy with a b c
+      rw [tlift_injective b, tlift_injective c]
+      simp_all only [Fin.mk.injEq, DecisionTree.branch.injEq, and_self, and_true]
+      ext
+      simp_all only
+
+private lemma olift_preserves_toTree {h : n ≤ n'} {O : OBdd n m} : (olift h O).toTree = tlift h O.toTree := by
+  cases O_root_def : O.1.root with
+  | terminal b =>
+    simp only [OBdd.toTree_terminal' O_root_def, tlift, olift, lift]
+    simp_rw [O_root_def, OBdd.toTree_terminal]
+  | node j =>
+    simp only [OBdd.toTree_node O_root_def, tlift]
+    rw [← olift_preserves_toTree (h := h) (O := (O.low  O_root_def))]
+    rw [← olift_preserves_toTree (h := h) (O := (O.high O_root_def))]
+    rw [← olift_preserves_root (h := h)] at O_root_def
+    simp only [OBdd.toTree_node O_root_def]
+    simp only [DecisionTree.branch.injEq]
+    constructor
+    · simp [olift]
+    · constructor
+      · rw [olift_low]
+      · rw [olift_high]
+termination_by O
+
+private lemma tlift_evaluate {h : n ≤ n'} {T : DecisionTree n} {I : Vector Bool n'} :
+    (tlift h T).evaluate I = T.evaluate (Vector.cast (show (min n n') = n by simpa) (I.take n)) := by
+  cases T with
+  | leaf => simp [tlift, DecisionTree.evaluate]
+  | branch _ _ _ =>
+    simp only [tlift, DecisionTree.evaluate]
+    rw [tlift_evaluate]
+    rw [tlift_evaluate]
+    refine ite_congr ?_ (congrFun rfl) (congrFun rfl)
+    simp only [eq_iff_iff, Bool.coe_iff_coe, Fin.getElem_fin]
+    rename_i a _ _
+    have : (I.take n)[a.1] = I[a.1] := by
+      apply Vector.getElem_take
+    rw [← this]
+    rfl
+
+@[simp]
+lemma olift_evaluate {h : n ≤ n'} {O : OBdd n m} {I : Vector Bool n'} :
+    (olift h O).evaluate I = O.evaluate (Vector.cast (show (min n n') = n by simpa) (I.take n)) := by
+  simp only [OBdd.evaluate, Function.comp_apply, olift_preserves_toTree]
+  rw [tlift_evaluate]
+
+lemma olift_SimilarRP {h : n ≤ n'} {O : OBdd n m} {p q : Pointer m}
+    {hp : Pointer.Reachable (olift h O).1.heap (olift h O).1.root p}
+    {hq : Pointer.Reachable (olift h O).1.heap (olift h O).1.root q} :
+    (olift h O).SimilarRP ⟨p, hp⟩ ⟨q, hq⟩ →
+    O.SimilarRP ⟨p, (lift_reachable_iff (h := h)).mpr hp⟩ ⟨q, (lift_reachable_iff (h := h)).mpr hq⟩ := by
+  intro sim
+  simp only [OBdd.SimilarRP, OBdd.Similar, OBdd.HSimilar] at sim
+  have : OBdd.toTree ⟨{heap := (olift h O).1.heap, root := p}, Bdd.ordered_of_reachable hp⟩ = OBdd.toTree (olift h ⟨{heap := O.1.heap, root := p}, Bdd.ordered_of_reachable (lift_reachable_iff.mpr hp)⟩) := by
+    rfl
+  rw [this] at sim
+  have : OBdd.toTree ⟨{heap := (olift h O).1.heap, root := q}, Bdd.ordered_of_reachable hq⟩ = OBdd.toTree (olift h ⟨{heap := O.1.heap, root := q}, Bdd.ordered_of_reachable (lift_reachable_iff.mpr hq)⟩) := by
+    rfl
+  rw [this] at sim
+  rw [olift_preserves_toTree] at sim
+  rw [olift_preserves_toTree] at sim
+  clear this
+  clear this
+  simp only [OBdd.SimilarRP, OBdd.Similar,OBdd.HSimilar]
+  rw [tlift_injective sim]
+
+lemma olift_reduced {n n' m : Nat} {h : n ≤ n'} {O : OBdd n m} : O.Reduced → (olift h O).Reduced := by
+  rintro ⟨r1, r2⟩
+  constructor
+  · exact NoRedundancy_of_olift r1
+  · rintro _ _ sim; exact r2 (olift_SimilarRP sim)
+
+end Lift
